Attempt to re-enable join conditions meta-opt

Optimizations/DSL/MetaOptimization.thy
@@ -2,6 +2,59 @@ theory MetaOptimization
   imports CodeGenAltAlt
 begin
 
+context includes match_syntax match_pattern_syntax begin
+lemma eval_match_equivalence:
+  assumes "\<forall>e. (m \<U> \<sigma> = e) = (m' \<U> \<sigma> = e)"
+  shows "eval_match m \<sigma> = eval_match m' \<sigma>"
+  using assms
+  by blast
+
+lemma eval_match_redundant:
+  assumes "valid_match m"
+  shows "eval_match (m && m) u = eval_match m u"
+  using assms AndThen eval_match_andthen eval_match_deterministic eval_match_idempotent eval_match_equivalence
+  by (smt (verit, del_insts))
+
+lemma eval_rules_choice_map_induct:
+  assumes "eval_rules (a) u e = eval_rules (f a) u e"
+  assumes "eval_rules (choice rules) u e = eval_rules (choice (map f rules)) u e"
+  shows "eval_rules (choice (a # rules)) u e = eval_rules (choice (map f (a # rules))) u e"
+  using assms choiceE eval_rules.intros(5,6,7)
+  by (smt (verit, ccfv_threshold) list.map_disc_iff list.set_intros(1) list.set_intros(2) list.simps(9) option.distinct(1) set_ConsD)
+
+lemma monotonic_cond:
+  assumes "\<forall>e u. eval_rules r u e = eval_rules (f r) u e"
+  shows "\<forall>e u. eval_rules (m ? r) u e = eval_rules (m ? f r) u e"
+  using assms by (metis condE eval_rules.intros(2))
+
+lemma monotonic_else:
+  assumes "\<forall>e u. eval_rules r1 u e = eval_rules (f r1) u e"
+  assumes "\<forall>e u. eval_rules r2 u e = eval_rules (f r2) u e"
+  shows "\<forall>e. eval_rules (r1 else r2) u e = eval_rules (f r1 else f r2) u e"
+  using assms
+  by (metis elseE eval_rules.intros(3) eval_rules.intros(4))
+
+lemma monotonic_seq_with_entry:
+  assumes "\<forall>e u. eval_rules r1 u e = eval_rules (f r1) u e"
+  assumes "\<forall>e u. eval_rules r2 u e = eval_rules (f r2) u e"
+  assumes "entry_var r2 = entry_var (f r2)"
+  shows "\<forall>e. eval_rules (r1 \<Zsemi> r2) u e = eval_rules (f r1 \<Zsemi> f r2) u e"
+  using assms seqE
+  by (smt (verit, ccfv_SIG) eval_rules.intros(10) eval_rules.intros(8) eval_rules.intros(9))
+
+lemma monotonic_seq_without_entry:
+  assumes "\<forall>e u. eval_rules r1 u e = eval_rules (f r1) u e"
+  shows "\<forall>e. eval_rules (r1 \<Zsemi> r2) u e = eval_rules ((f r1) \<Zsemi> r2) u e"
+  using assms seqE
+  by (smt (verit, ccfv_SIG) eval_rules.intros(10) eval_rules.intros(8) eval_rules.intros(9))
+
+lemma monotonic_choice:
+  assumes "\<forall>r e u. r \<in> set rules \<longrightarrow> eval_rules r u e = eval_rules (f r) u e"
+  shows "\<forall>e. eval_rules (choice rules) u e = eval_rules (choice (map f rules)) u e"
+  using assms apply (induction rules) apply simp
+  by (metis eval_rules_choice_map_induct list.set_intros(1) list.set_intros(2))
+end
+
 
 section \<open>Meta-optimizations\<close>
 
@@ -139,14 +192,20 @@ definition run :: "Rules \<Rightarrow> Rules" where
 end
 
 
-context includes match_syntax match_pattern_syntax
-begin
+context includes match_syntax match_pattern_syntax begin
 subsection \<open>Lift Match Sequence to Rule Conditions\<close>
 
 fun lift_cond :: "Rules \<Rightarrow> Rules option" where
   "lift_cond ((m1 && m2) ? r) = (Some (m1 ? (m2 ? r)))" |
   "lift_cond _ = None"
 
+lemma lift_condE:
+  "lift_cond r = Some r' \<Longrightarrow> \<exists>m1 m2 rule. r = ((m1 && m2) ? rule) \<and> r' = (m1 ? (m2 ? rule))"
+  apply (cases r) apply auto 
+  subgoal for cond 
+    apply (cases cond) by auto
+  done
+  
 lemma lift_cond_sound:
   "eval_rules ((m1 && m2) ? r) \<sigma> = eval_rules (m1 ? (m2 ? r)) \<sigma>"
 proof -
@@ -182,22 +241,13 @@ setup \<open>Locale_Code.open_block\<close>
 interpretation lift_cond : metaopt
   lift_cond
   combined_size
-  apply standard
-  using lift_cond_sound apply auto sorry (*
-  subgoal for rules apply (induction rules; auto)
-  using lift_cond.elims sledgehammer
-  apply (metis lift_cond.elims option.distinct(1) option.inject)*)
-(*
-  subgoal for rules apply (induction rules; auto)
-  using lift_cond.elims option.distinct(1) option.sel sledgehammer
-  by (smt (verit))
-    by (smt (verit) lift_cond.elims option.distinct(1) option.sel)
-  apply (smt (verit) lift_cond.elims option.distinct(1) option.sel)
-        apply (smt (verit) lift_cond.elims option.distinct(1) option.sel)
-  using combined_size_decreases lift_cond.elims apply force
-      apply simp
-  subgoal for rules apply (induction rules; auto) done
-  by simp+*)
+  apply standard apply auto
+  using lift_cond_sound lift_condE apply blast
+  using combined_size_decreases lift_condE apply blast
+  subgoal for rules r apply (induction rules) 
+    apply fastforce
+    by force
+  done
 setup \<open>Locale_Code.close_block\<close>
 
 fun run where "run x = lift_cond.apply_meta x"
@@ -342,5 +392,584 @@ value "reduce (snd (Predicate.the (generateC STR ''myrule''
     (BinaryExprPattern BinSub (BinaryExprPattern BinAdd (VariableExprPattern STR ''x'') (VariableExprPattern STR ''y'')) (VariableExprPattern STR ''x''))
     None
     (VariableExprPattern STR ''x''))))"
+
+
+
+subsection \<open>Join Shared Conditions\<close>
+
+context includes match_syntax match_pattern_syntax begin
+(*fun common_size :: "Rules \<Rightarrow> nat" where
+  "common_size (m ? r) = 1 + common_size r" |
+  "common_size (base l e) = 0" |
+  "common_size (r1 else r2) = 1 + common_size r1 + common_size r2" |
+  "common_size (choice (rule # rules)) = 1 + common_size rule + common_size (choice rules)" |
+  "common_size (choice []) = 0" |
+  "common_size (r1 \<Zsemi> r2) = 1 + common_size r1 + common_size r2"
+*)
+
+fun find_common :: "MATCH \<Rightarrow> Rules \<Rightarrow> Rules option" where
+  "find_common m (m' ? r) = (if m = m' then Some r else None)" |
+  "find_common m r = None"
+
+fun find_uncommon :: "MATCH \<Rightarrow> Rules \<Rightarrow> Rules option" where
+  "find_uncommon m (m' ? r) = (if m = m' then None else Some (m' ? r))" |
+  "find_uncommon m r = Some r"
+
+definition join_common :: "MATCH \<Rightarrow> Rules list \<Rightarrow> Rules list" where
+  "join_common m rules = List.map_filter (find_common m) rules"
+
+definition join_uncommon :: "MATCH \<Rightarrow> Rules list \<Rightarrow> Rules list" where
+  "join_uncommon m rules = List.map_filter (find_uncommon m) rules"
+
+lemma find_common_defn:
+  assumes "find_common m x = v"
+  shows "v \<noteq> None \<longleftrightarrow> (\<exists>r. x = (m ? r) \<and> v = Some r)"
+  using assms apply (induction m x rule: find_common.induct) unfolding find_common.simps apply force
+  by simp+
+
+lemma find_uncommon_preserve:
+  "find_uncommon m r = Some r \<or> find_uncommon m r = None"
+  by (metis find_uncommon.elims)
+
+lemma join_uncommon_subset:
+  "set (join_uncommon m x) \<subseteq> set x"
+  unfolding join_uncommon_def List.map_filter_def using find_uncommon_preserve
+  by (smt (verit, best) comp_def filter_is_subset list.map_ident_strong mem_Collect_eq option.sel set_filter)
+
+fun combine_conditions :: "Rules \<Rightarrow> Rules option" where
+  "combine_conditions (choice ((m ? r) # rules)) = 
+    Some 
+      (choice ((m ? (choice (r # join_common m rules)))
+        # [(choice (join_uncommon m rules))]))" |
+  "combine_conditions _ = None"
+
+lemma join_common_empty: "join_common m [] = []"
+  by (simp add: join_common_def map_filter_simps(2))
+lemma join_uncommon_empty: "join_uncommon m [] = []"
+  by (simp add: join_uncommon_def map_filter_simps(2))
+
+lemma eval_choice: "{e. eval_rules (choice rules) u e \<and> e \<noteq> None} = {e | e r . r \<in> set rules \<and> eval_rules r u e \<and> e \<noteq> None}"
+  using choiceE eval_rules.intros(5) by fastforce
+
+lemma eval_choice_none: "eval_rules (choice rules) u None = (\<forall> r \<in> set rules . eval_rules r u None)"
+  by (metis choiceE eval_rules.intros(6) length_pos_if_in_set list.size(3) nless_le option.distinct(1))
+
+inductive_cases evalRulesE: "eval_rules r u e"
+
+lemmas monotonic =
+  monotonic_cond
+  monotonic_else
+  monotonic_choice
+  monotonic_seq_with_entry
+  monotonic_seq_without_entry
+
+lemma unordered_choice:
+  assumes "set rules = set rules'"
+  shows "\<forall>e. eval_rules (choice rules) u e = eval_rules (choice rules') u e"
+  using assms by (metis choiceE eval_choice_none eval_rules.intros(5))
+
+lemma find_inverse_lhs:
+  "\<exists>e. find_common m rules = None \<longleftrightarrow> find_uncommon m rules = Some e"
+  by (smt (verit, best) find_common.elims find_uncommon.simps(1) find_uncommon.simps(2) find_uncommon.simps(3) find_uncommon.simps(4) find_uncommon.simps(5))
+
+lemma find_inverse_rhs:
+  "\<exists>e. find_common m rules = Some e \<longleftrightarrow> find_uncommon m rules = None"
+  by (smt (verit, best) find_common.elims find_uncommon.simps(1) find_uncommon.simps(2) find_uncommon.simps(3) find_uncommon.simps(4) find_uncommon.simps(5))
+
+lemma join_common_equal:
+  assumes "find_common m a = None"
+  shows "(map ((?) m) (join_common m rules')) = (map ((?) m) (join_common m (a # rules')))"
+  apply (simp add: join_common_def join_uncommon_def List.map_filter_def)
+  by (simp add: assms)
+
+lemma join_common_plus:
+  assumes "find_common m a = Some a'"
+  shows "(m ? a') # (map ((?) m) (join_common m rules')) = (map ((?) m) (join_common m (a # rules')))"
+  using assms unfolding join_common_def join_uncommon_def List.map_filter_def
+  by simp
+
+lemma join_combines:
+  "(set (map (\<lambda>r. m ? r) (join_common m rules)) \<union> set (join_uncommon m rules)) = set rules"
+  apply (induction rules) 
+    apply (simp add: join_common_def join_uncommon_def List.map_filter_def)
+  subgoal premises induct for a rules'
+  proof (cases "find_common m a")
+    case None
+    have "find_uncommon m a = Some a" 
+      using None find_inverse_lhs
+      by (metis find_uncommon_preserve option.distinct(1))
+    then have "join_uncommon m (a # rules') = a # (join_uncommon m rules')"
+      unfolding join_common_def join_uncommon_def List.map_filter_def
+      by simp
+    then show ?thesis using induct join_common_equal
+      by (metis None Un_insert_right list.simps(15))
+  next
+    case (Some a')
+    have "find_uncommon m a = None" 
+      by (metis Some find_common_defn find_uncommon.simps(1) option.distinct(1))
+    then have "join_uncommon m (a # rules') = (join_uncommon m rules')"
+      unfolding join_common_def join_uncommon_def List.map_filter_def
+      by simp
+    then show ?thesis
+      by (metis Some Un_insert_left find_common.elims induct join_common_plus list.simps(15) option.distinct(1))
+  qed
+  done
+
+lemma join_common_set_def:
+  "set (join_common m rules) = {r. (m ? r) \<in> set rules}"
+  unfolding join_common_def List.map_filter_def 
+  apply (induction rules)
+   apply simp 
+  subgoal for a rules 
+    apply (cases a) by auto
+  done
+
+lemma join_uncommon_set_def:
+  "set (join_uncommon m rules) = {r. r \<in> set rules \<and> (\<forall>r'. r \<noteq> (m ? r'))}"
+  unfolding join_uncommon_def List.map_filter_def 
+  apply (induction rules) apply simp
+  subgoal for a rules 
+    apply (cases a) by auto
+  done
+
+lemma
+  assumes "\<exists>r \<in> set rules. r \<in> set rules' \<and> eval_rules r u (Some e)"
+  shows "eval_rules (choice rules) u (Some e) = eval_rules (choice rules') u (Some e)"
+  using assms
+  using eval_rules.intros(5) by blast
+
+lemma map_None:
+  "(\<forall>r\<in>set rules. eval_rules (m ? r) u None) = eval_rules (choice (map ((?) m) rules)) u None"
+  (is "?lhs = eval_rules ?rhs u None")
+proof -
+  have setequiv: "set (map ((?) m) rules) = {m ? r | r . r\<in>set rules}"
+    by (simp add: Setcompr_eq_image)
+  then show ?thesis
+    using eval_choice_none by auto
+qed
+
+lemma setequiv: "set (map ((?) m) rules) = {m ? r | r . r\<in>set rules}"
+  by (simp add: Setcompr_eq_image)
+
+lemma eval_rules_cond_fail:
+  assumes "\<not>(\<exists>e. eval_match m u e)"
+  shows "\<not>(eval_rules (m ? r) u e)"
+  using assms
+  by (meson condE)
+
+lemma eval_rules_choice_fail:
+  assumes "\<not>(\<exists>e. eval_match m u e)"
+  assumes "rules \<noteq> []"
+  shows "\<not>(eval_rules (choice (map ((?) m) rules)) u e)" (is "\<not>(eval_rules (choice ?rules) u e)")
+proof -
+  have "\<forall>r \<in> set ?rules. \<not>(eval_rules (r) u e)"
+    by (simp add: assms eval_rules_cond_fail)
+  then show ?thesis
+    using assms choiceE
+    by (smt (verit) condE list.set_intros(1) map_None neq_Nil_conv)
+qed
+
+(*
+lemma eval_rules_choice_empty:
+  assumes "eval_rules (choice []) u e"
+  shows "eval_rules (m ? choice []) u e"
+proof -
+  have "eval_rules (choice []) u None"
+    by (simp add: eval_rules.intros(7))
+  have "eval_rules (m ? choice []) u None"
+    sledgehammer
+  then show "eval_rules (m ? choice []) u e"
+    sledgehammer
+
+lemma pull_cond_out_rhs:
+  assumes "eval_rules (choice (map ((?) m) rules)) u e" (is "eval_rules ?lhs u e")
+  shows "eval_rules (m ? choice rules) u e" (is "eval_rules ?rhs u e")
+proof (cases rules)
+  case Nil
+  then show ?thesis using assms sledgehammer
+next
+  case (Cons a list)
+  then show ?thesis sorry
+qed
+  proof (cases "\<not>(\<exists>e. eval_match m u e)")
+    case True \<comment> \<open>If m doesn't match then both the lhs and rhs should evaluate to e = None\<close>
+    have lhs: "\<forall>e. eval_rules ?lhs u e \<longrightarrow> e = None"
+      using True eval_rules.intros(2) eval_rules.intros(5)
+      by (smt (verit, del_insts) choiceE condE ex_map_conv option.distinct(1))
+    have rhs: "\<forall>e. eval_rules ?rhs u e \<longrightarrow> e = None"
+      by (meson True condE)
+    then show ?thesis using assms condE
+      using lhs rhs sledgehammer
+      using eval_always_result
+      using assms by blast
+  next
+    case match: (Some a) \<comment> \<open>Drop down into evaluation post matching m\<close>
+      have allEval: "\<forall>r \<in> set rules. eval_rules r a e = eval_rules (m ? r) u e"
+        by (metis match condE eval_rules.intros(2) option.distinct(1) option.sel)
+        then show ?thesis
+        proof (cases e)
+          case evalsNone: None
+          have "\<forall>r \<in> set rules. eval_rules r a None"
+            using evalsNone allEval assms map_None by blast
+          then have "\<forall>r \<in> set rules. eval_rules (m ? r) u None"
+            using evalsNone allEval by blast
+          then have "eval_rules ?lhs u None"
+            by (simp add: map_None)
+          then show ?thesis
+            using evalsNone
+            using \<open>\<forall>r\<in>set rules. eval_rules r a None\<close> eval_choice_none eval_rules.intros(2) match by blast
+        next
+          case evalsSome: (Some a')
+            then have "\<exists>r \<in> set rules. eval_rules (m ? r) u (Some a')"
+              using condE assms match
+              using choiceE by fastforce
+            then have "\<exists>r \<in> set rules. eval_rules (m ? r) u e"
+              by (simp add: evalsSome)
+            then have "eval_rules ?rhs u e"
+              using allEval eval_rules.intros(2) eval_rules.intros(6) evalsSome match by blast
+            then show ?thesis
+              by simp
+          qed
+        qed
+
+lemma pull_cond_out_lhs:
+  assumes "eval_rules (m ? choice rules) u e" (is "eval_rules ?lhs u e")
+  shows "eval_rules (choice (map ((?) m) rules)) u e" (is "eval_rules ?rhs u e")
+  proof (cases "eval_match m u")
+    case None \<comment> \<open>If m doesn't match then both the lhs and rhs should evaluate to e = None\<close>
+    have lhs: "\<forall>e. eval_rules ?lhs u e \<longrightarrow> e = None"
+      using None eval_rules.intros(3) eval_rules.intros(7)
+      by (smt (verit, del_insts) choiceE condE ex_map_conv option.distinct(1))
+    have rhs: "\<forall>e. eval_rules ?rhs u e \<longrightarrow> e = None"
+      by (simp add: lhs pull_cond_out_rhs)
+    then show ?thesis using lhs rhs
+      using eval_always_result
+      using assms by blast
+  next
+    case match: (Some a) \<comment> \<open>Drop down into evaluation post matching m\<close>
+      have allEval: "\<forall>r \<in> set rules. eval_rules r a e = eval_rules (m ? r) u e"
+        by (metis match condE eval_rules.intros(2) option.distinct(1) option.sel)
+        then show ?thesis
+        proof (cases e)
+          case evalsNone: None
+          have "\<forall>r \<in> set rules. eval_rules r a None"
+            by (metis assms condE eval_choice_none evalsNone match option.discI option.inject)
+          then have "\<forall>r \<in> set rules. eval_rules (m ? r) u None"
+            using evalsNone allEval by blast
+          then show ?thesis
+            using evalsNone map_None by blast
+        next
+          case evalsSome: (Some a')
+            then have "\<exists>r \<in> set rules. eval_rules (m ? r) u (Some a')"
+              using condE assms match
+              using choiceE
+              by (metis allEval option.distinct(1) option.sel)
+            then have "\<exists>r \<in> set rules. eval_rules (m ? r) u e"
+              by (simp add: evalsSome)
+            then have "eval_rules ?rhs u e"
+              by (metis eval_rules.intros(6) evalsSome image_eqI image_set)
+            then show ?thesis
+              by simp
+          qed
+        qed
+
+lemma pull_cond_out:
+  "eval_rules (choice (map ((?) m) rules)) u e = eval_rules (m ? choice rules) u e"
+  using pull_cond_out_lhs pull_cond_out_rhs by blast
+
+lemma cases_None:
+  assumes "eval_rules (choice ((m ? r) # rules)) u None"
+  shows "
+  eval_rules (m ? (choice (r # join_common m rules))) u None \<and>
+  eval_rules ((choice (join_uncommon m rules))) u None"
+  apply (rule conjI)
+  using assms
+  unfolding join_common_def List.map_filter_def
+   apply (induction rules) apply simp using pull_cond_out
+    apply fastforce apply auto[1] using pull_cond_out defer defer
+    apply (meson assms eval_choice_none join_uncommon_subset list.set_intros(2) subsetD)
+  subgoal for a rules y
+    apply (cases a)
+        apply force
+    subgoal premises pre for m' r' 
+    proof -
+      have "m = m'"
+        using pre(3,4)
+        by (metis find_common.simps(1) option.distinct(1))
+      then show ?thesis using pre apply auto[1]
+        by (smt (verit, del_insts) eval_choice_none list.set_intros(1) list.set_intros(2) list.simps(9) pull_cond_out set_ConsD)
+    qed
+      by simp+
+  subgoal for a rules
+    apply (cases a)
+    by (simp add: eval_choice_none)+
+  done
+
+lemma cases_None1:
+  assumes "
+  eval_rules (m ? (choice (r # join_common m rules))) u None \<and>
+  eval_rules ((choice (join_uncommon m rules))) u None"
+  shows "eval_rules (choice ((m ? r) # rules)) u None"
+proof -
+  have head: "eval_rules (m ? r) u None"
+    using assms
+    by (meson list.set_intros(1) map_None pull_cond_out_lhs)
+  have common_None: "\<forall>r' \<in> set (join_common m rules). eval_rules (m ? r') u None"
+    by (meson assms list.set_intros(2) map_None pull_cond_out_lhs)
+  have uncommon_None: "\<forall>r' \<in> set (join_uncommon m rules). eval_rules r' u None"
+    using assms eval_choice_none by blast
+  have "\<forall>r' \<in> set rules. eval_rules r' u None"
+    using join_combines common_None uncommon_None pull_cond_out
+    by (metis (no_types, lifting) UnE assms eval_choice_none list.set_intros(2) list.simps(9))
+  then show ?thesis using head
+    by (simp add: eval_choice_none)
+qed
+
+  
+lemma cases_Some:
+  assumes "eval_rules (choice rules) u (Some e)"
+  shows "
+  eval_rules (m ? (choice (join_common m rules))) u (Some e) \<or>
+  eval_rules ((choice (join_uncommon m rules))) u (Some e)"
+proof -
+  obtain r where r: "r \<in> set rules \<and> eval_rules r u (Some e)"
+    by (metis assms choiceE option.discI)
+  then show ?thesis
+  proof (cases r)
+    case (base x1)
+    have "r \<in> set (join_uncommon m rules)"
+      using join_uncommon_set_def base r by blast
+    then show ?thesis
+      using eval_rules.intros(6) r by presburger
+  next
+    case (cond m' r')
+    then show ?thesis
+    proof (cases "m = m'")
+      case True
+      then have "r' \<in> set (join_common m rules)"
+        using cond r join_common_set_def
+        by blast
+      then show ?thesis
+        by (metis True cond eval_rules.intros(6) image_eqI image_set pull_cond_out_rhs r)
+    next
+      case False
+      have "r \<in> set (join_uncommon m rules)"
+        using join_uncommon_set_def False r
+        using cond by blast
+      then show ?thesis
+        using eval_rules.intros(6) r by presburger
+    qed
+  next
+    case (else x31 x32)
+    have "r \<in> set (join_uncommon m rules)"
+      using join_uncommon_set_def else r by blast
+    then show ?thesis
+      using eval_rules.intros(6) r by presburger
+  next
+    case (seq x41 x42)
+    have "r \<in> set (join_uncommon m rules)"
+      using join_uncommon_set_def seq r by blast
+    then show ?thesis
+      using eval_rules.intros(6) r by presburger
+  next
+    case (choice x5)
+    have "r \<in> set (join_uncommon m rules)"
+      using join_uncommon_set_def choice r by blast
+    then show ?thesis
+      using eval_rules.intros(6) r by presburger
+  qed
+qed
+
+lemma cases_Some1:
+  assumes "eval_rules (choice ((m ? r) # rules)) u (Some e)"
+  shows "
+  eval_rules (m ? (choice (r # join_common m rules))) u (Some e) \<or>
+  eval_rules ((choice (join_uncommon m rules))) u (Some e)"
+  using cases_Some assms
+  by (smt (verit, ccfv_threshold) choiceE eval_rules.intros(6) list.set_intros(1) list.set_intros(2) list.simps(9) option.distinct(1) pull_cond_out set_ConsD)
+
+lemma cases_Some2:
+  assumes "eval_rules (m ? (choice (r # join_common m rules))) u (Some e) \<or>
+  eval_rules ((choice (join_uncommon m rules))) u (Some e)" (is "?c1 \<or> ?c2")
+  shows "eval_rules (choice ((m ? r) # rules)) u (Some e)"
+using assms proof (rule disjE)
+  assume c1: "?c1"
+  then show ?thesis
+  proof (cases "eval_rules (m ? r) u (Some e)")
+    case True
+    then show ?thesis
+      by (meson eval_rules.intros(6) list.set_intros(1))
+  next
+    case False
+    then have "\<exists>r \<in>set (join_common m rules). eval_rules (m ? r) u (Some e)"
+      using c1
+      by (smt (verit, del_insts) choiceE condE eval_rules.intros(2) option.distinct(1) set_ConsD)
+    then show ?thesis 
+      by (metis eval_rules.intros(6) join_common_set_def list.set_intros(2) mem_Collect_eq)
+  qed
+next
+  assume "?c2"
+  then have "\<exists>r \<in>set (join_uncommon m rules). eval_rules r u (Some e)"
+    by (metis choiceE option.discI)
+  then show ?thesis
+    by (meson eval_rules.intros(6) join_uncommon_subset list.set_intros(2) subsetD)
+qed
+
+lemma evalchoice_twoelement:
+  assumes "eval_rules (choice [x1, x2]) u (Some e)"
+  shows "eval_rules x1 u (Some e) \<or> eval_rules x2 u (Some e)"
+  using assms choiceE by fastforce
+*)
+
+lemma combine_conditions_valid:
+  "combine_conditions r = Some r' \<Longrightarrow> eval_rules r u e = eval_rules r' u e"
+  apply (induction r arbitrary: u e r' rule: combine_conditions.induct) defer apply simp+
+  subgoal premises p for m r rules u e
+  proof (rule iffI)
+    assume eval: "eval_rules (choice ((m ? r) # rules)) u e"
+    show "eval_rules
+     (choice
+       [m ? (choice (r # join_common m rules)),
+        (choice (join_uncommon m rules))])
+     u e"
+    proof (cases e)
+      case None
+      have "eval_rules (m ? (choice (r # join_common m rules))) u None \<and>
+  eval_rules ((choice (join_uncommon m rules))) u None"
+        sorry
+        using None cases_None eval by blast
+      then have "eval_rules (m ? combine_conditions (choice (r # join_common m rules))) u None \<and>
+  eval_rules (combine_conditions (choice (join_uncommon m rules))) u None" 
+        using p monotonic_cond by blast
+      then show ?thesis using None eval_choice_none by simp
+    next
+      case (Some a)
+      have "eval_rules (m ? (choice (r # join_common m rules))) u (Some a) \<or>
+  eval_rules ((choice (join_uncommon m rules))) u (Some a)"
+        using Some cases_Some1 eval by simp
+      then have "eval_rules (m ? combine_conditions (choice (r # join_common m rules))) u (Some a) \<or>
+  eval_rules (combine_conditions (choice (join_uncommon m rules))) u (Some a)"
+        using p monotonic_cond by blast
+      then show ?thesis
+        by (metis Some eval_rules.intros(6) list.set_intros(1) list.set_intros(2))
+    qed
+  next
+    assume eval: "eval_rules
+     (choice
+       [m ? combine_conditions (choice (r # join_common m rules)),
+        combine_conditions (choice (join_uncommon m rules))])
+     u e"
+    show "eval_rules (choice ((m ? r) # rules)) u e"
+    proof (cases e)
+      case None
+      then have "eval_rules (m ? (choice (r # join_common m rules))) u None \<and>
+  eval_rules ((choice (join_uncommon m rules))) u None"
+        by (smt (verit) eval eval_choice_none list.set_intros(1) list.set_intros(2) monotonic_cond p(1) p(2))
+      then show ?thesis using cases_None1 None by blast
+    next
+      case (Some a)
+      then have "eval_rules (m ? combine_conditions (choice (r # join_common m rules))) u (Some a) \<or>
+  eval_rules (combine_conditions (choice (join_uncommon m rules))) u (Some a)"
+        using eval evalchoice_twoelement by simp
+      then have "eval_rules (m ? (choice (r # join_common m rules))) u (Some a) \<or>
+  eval_rules ((choice (join_uncommon m rules))) u (Some a)"
+        using p monotonic_cond by blast
+      then show ?thesis using cases_Some2 Some
+        by simp
+    qed
+  qed
+  done
+
+
+fun eliminate_choice :: "Rules \<Rightarrow> Rules" where
+  "eliminate_choice (base e) = base e" |
+  "eliminate_choice (r1 else r2) = (eliminate_choice r1 else eliminate_choice r2)" |
+  "eliminate_choice (m ? r) = (m ? eliminate_choice r)" |
+  "eliminate_choice (choice (r # [])) = eliminate_choice r" |
+  "eliminate_choice (choice rules) = 
+    choice (map eliminate_choice rules)" |
+  "eliminate_choice (r1 \<Zsemi> r2) = (eliminate_choice r1 \<Zsemi> eliminate_choice r2)"
+
+lemma choice_Single:
+  "eval_rules (choice [r]) u e = eval_rules r u e"
+  apply (cases e)
+  using eval_choice_none apply auto[1]
+  using choiceE eval_rules.intros(6) by fastforce
+
+lemma entry_var_single_choice:
+  "entry_var r = entry_var (choice [r])"
+  unfolding entry_var.simps by simp
+
+lemma entry_var_eliminate_choice:
+  "entry_var r = entry_var (eliminate_choice r)"
+  apply (induction r rule: eliminate_choice.induct)
+  apply simp 
+  using eliminate_choice.simps(2) entry_var.simps(3) apply presburger
+  using eliminate_choice.simps(3) entry_var.simps(1) apply presburger
+  unfolding eliminate_choice.simps
+  using entry_var_single_choice apply presburger
+  apply simp 
+  using entry_var_rules apply blast
+  using entry_var.simps(5) by presburger
+
+
+lemma eliminate_choice_valid_1:
+  "{e. eval_rules r u e} = {e. eval_rules (eliminate_choice r) u e}"
+  apply (induction r arbitrary: u rule: eliminate_choice.induct)
+  apply simp unfolding eliminate_choice.simps
+  apply (smt (verit) Collect_cong elseE eval_rules.intros(4) eval_rules.intros(5) mem_Collect_eq)
+  unfolding eliminate_choice.simps
+      apply (smt (verit) Collect_cong condE eval_rules.intros(3) eval_rules.simps mem_Collect_eq)
+  unfolding eliminate_choice.simps
+  using choice_Single apply presburger
+  using monotonic_choice apply blast
+  apply (metis Collect_cong mem_Collect_eq monotonic_choice)
+  using entry_var_eliminate_choice
+  by (smt (verit, ccfv_SIG) Collect_cong mem_Collect_eq monotonic_seq_with_entry)
+
+lemma eliminate_choice_valid:
+  "eval_rules r u e = eval_rules (eliminate_choice r) u e"
+  using eliminate_choice_valid_1 by blast
+
+definition optimized_export where
+  "optimized_export = eliminate_choice \<circ> combine_conditions o lift_common o lift_match o eliminate_noop"
+
+lemma elim_noop_preserve_def_vars:
+  "def_vars m = def_vars (elim_noop m)"
+  apply (induction m rule: elim_noop.induct) by simp+
+
+lemma elim_noop_preserve_use_vars:
+  "use_vars m = use_vars (elim_noop m)"
+  apply (induction m rule: elim_noop.induct) apply simp+
+  using elim_noop_preserve_def_vars by simp+
+
+lemma elim_noop_preserve_valid:
+  assumes "valid_match m"
+  shows "valid_match (elim_noop m)"
+    using assms apply (induction m rule: elim_noop.induct) apply simp+
+    using elim_noop_preserve_def_vars elim_noop_preserve_use_vars by simp+
+
+lemma eliminate_noop_preserve_valid:
+  assumes "valid_rules r"
+  shows "valid_rules (eliminate_noop r)"
+  using assms apply (induction r rule: eliminate_noop.induct) apply simp
+  apply (simp add: elim_noop_preserve_valid) by simp+
+
+
+lemma lift_match_preserve_valid:
+  assumes "valid_rules r"
+  shows "valid_rules (lift_match r)"
+  using assms apply (induction r rule: lift_match.induct) apply simp
+  by simp+
+
+lemma optimized_export_valid:
+  assumes "valid_rules r"
+  shows "eval_rules r u e = eval_rules (optimized_export r) u e"
+  unfolding optimized_export_def comp_def
+  using lift_common_valid lift_match_valid eliminate_noop_valid 
+  using combine_conditions_valid eliminate_choice_valid
+  by (metis assms eliminate_noop_preserve_valid lift_match_preserve_valid)
+
+thm_oracles optimized_export_valid
 
 end
